

\begin{align}
	\|\vb{r}_{j}^{(k)}\|_{B^{-1}} = \|\vb{b} - (A + \sigma_{k}B)\vb{x}_{j}\|_{B^{-1}}
		&= \|\vb{b} - (A + \sigma B)W_{j}\vb{z}_{j} \|_{B^{-1}} \notag \\
		&= \left\| \norm{\vb{b}}_{B^{-1}}BW_{j+1}\vb{e}_{1} - BW_{j+1}\hat{T}_{j}^{(k)} \vb{z}_{j} \right\|_{B^{-1}} \notag \\
		&= \left\| BW_{j+1} \left( \norm{\vb{b}}_{B^{-1}}\vb{e}_1 - \hat{T}_{j}^{(k)} \vb{z}_{j} \right) \right\|_{B^{-1}} \notag \\
		&= \left\| \norm{\vb{b}}_{B^{-1}}\vb{e}_1 - \hat{T}_{j}^{(k)} \vb{z}_{j} \right\|_2
		\label{residual}
\end{align}
これは式\eqref{03-siki}